{-# OPTIONS --safe --without-K #-}

open import Level

module Functions.Laws (ℓ : Level) where

open import Function.Equivalence hiding (id; _∘_)
open import Data.Product using (_,_)

open import Categorical.Raw
     hiding (Category; Cartesian; Monoid; CartesianClosed; Logic)
open import Categorical.Laws
open import Categorical.Equiv
open import Functions.Raw ℓ public
open import Axiom.Extensionality.Propositional
open import Relation.Binary.PropositionalEquality
     renaming ( refl to refl≡
              ; trans to trans≡
              ; sym to sym≡
              )

module →-laws-instances where

  instance

    category : Category _⇾_
    category = record
      { identityˡ = λ _ → refl≡
      ; identityʳ = λ _ → refl≡
      ; assoc     = λ _ → refl≡
      ; ∘≈        = λ { {f = f}{k = k} h≈k f≈g x →
                      trans≡ (h≈k (f x)) (cong k (f≈g x)) }
      }

    cartesian : Cartesian _⇾_
    cartesian = record
      { ∀⊤ = λ _ → refl≡
      ; ∀× = equivalence
          (λ k≈f▵g → (λ x → cong exl (k≈f▵g x)) , (λ x → cong exr (k≈f▵g x)))
          (λ (exl∘k≈f , exr∘k≈g) x → cong₂ _,_ (exl∘k≈f x) (exr∘k≈g x))
      ; ▵≈ = λ h≈k f≈g x → cong₂ _,_ (h≈k x) (f≈g x)
      }

    -- -- I don't think this one can be proved without extensionality.
    -- indexedCartesian : ∀ {I : Set ℓ} → IndexedCartesian I _⇾_
    -- indexedCartesian = record
    --   { ∀Π = equivalence
    --       (λ k≈△fs i x → cong (λ f → f i) (k≈△fs x))
    --       (λ eqs x → {!!})
    --   ; △≈ = λ eqs x → {!!}
    --   }

    module ccc (extensionality : Extensionality _ _) where

      cartesianClosed : CartesianClosed _⇾_
      cartesianClosed = record
        { ∀⇛ = equivalence
            (λ g≈f (x , y) → sym≡ (cong (λ h → h y) (g≈f x)))
            (λ f≈uncurry-g x → extensionality λ y → sym≡ (f≈uncurry-g (x , y)))
        ; curry≈ = λ f≈g x → extensionality λ y → f≈g (x , y)
        }

    open import HasAlgebra

    -- monoid : ∀ {A : Set ℓ} ⦃ _ : HasMonoid A ⦄ → Monoid _⇾_
    -- monoid = record
    --   { ⟨∙⟩-identityˡ = λ (tt , _) → ∙-identityˡ
    --   ; ⟨∙⟩-identityʳ = λ (_ , tt) → ∙-identityʳ
    --   ; ⟨∙⟩-assoc = λ _ → ∙-assoc 
    --   }

    logic : Logic _⇾_
    logic = record { f∘cond = λ { (𝕗 , _) → refl≡ ; (𝕥 , _) → refl≡ } }
